src/PlutusIR/Semantics/Static/Theorems/Weakening.v
@@ -94,6 +94,12 @@ Module Typing.
     all: try (intros Delta'_0 Gamma'_0 HinclD HinclG).
     all: try (intros Delta'_0 HinclD).
     all: try solve [econstructor; subst; eauto using Kinding.weakening, inclusion_cons, inclusion_append].
+    - (* TyAbs *)
+      unfold P_has_type in H0.
+      apply T_TyAbs.
+      apply H0.
+      apply inclusion_cons; auto.
+      eapply drop_ty_var__inclusion_preserving; eauto.
     - (* T_Let NonRec*)
       econstructor; subst; eauto using Kinding.weakening, inclusion_cons, inclusion_append.
       apply Kinding.weakening with (Delta := drop_Δ Δ bs); auto.
